.

src/complexity/basic.lean
@@ -3,7 +3,10 @@ import tactic
 namespace complexity
 
 structure model :=
-  (Program Data Result Cost: Type*)
+  (Program: Type)
+  (Data: Type)
+  (Result: Type)
+  (Cost: Type)
   (data_equiv: setoid Data)
   (result_equiv: setoid Result)
   (cost_lt: preorder Cost)
@@ -32,7 +35,7 @@ theorem encode_inj_iff {α: Type*} {Data: Type*} [setoid Data] [has_encoding α 
   {a b: α}: ⟦(encode a:Data)⟧ = ⟦encode b⟧ ↔ a = b := ⟨ encode_inj, λ h, h ▸ rfl ⟩
 
 inductive witness
-  (m: complexity.model): Π {α β: Type*}, m.Program → α → β → Prop
+  (m: complexity.model): Π {α: Type*} {β: Type*}, m.Program → α → β → Prop
 | result {α: Type*} [complexity.has_encoding α m.Result] (p: m.Program) (c: m.Cost) (ret: α)
   (hc: m.has_cost p c) (hr: (m.result hc) = complexity.encode ret): witness p ret c
 | apply {α: Type*} {β: Type*} {γ: Type*} [complexity.has_encoding α m.Data] (p: m.Program) (f: α → β) (fc: α → γ)
@@ -40,6 +43,5 @@ inductive witness
 
 end complexity
 
-structure complexity {α β: Type*} (m: complexity.model) (f: α) (cost: β) :=
-  (program: m.Program)
-  (pf: complexity.witness m program f cost)
+def complexity {α: Type*} {β: Type*} (m: complexity.model) (f: α) (cost: β): Prop :=
+  ∃ (program: m.Program), complexity.witness m program f cost
